proof/correctness/R256.ec
@@ -1,5 +1,5 @@
-require import List Int IntExtra IntDiv CoreMap.
-from Jasmin require  import JModel.
+require import List Int IntExtra IntDiv CoreMap IntDiv.
+from Jasmin require  import JModel JMemory.
 
 require import Poly.
 require import Fq.
@@ -22,10 +22,9 @@ clone include PolyQPrincipalIdeal
 
 end R256.
 
-(*
 theory KyberPoly.
 
-clone import Z_3329_X__X_256.
+clone import R256.
 import Fq.
 import ZModP.
 
@@ -36,10 +35,11 @@ op q = W16.of_int 3329 axiomatized by qE.
 op add (a b : W16.t) = (a + b).
 
 op bw16 (a : W16.t) i =
-     (* 0 <= *) i < 14 /\ 
+     0 <= i <= 15 /\ (* signed 15 bits at most *)
      -2^i <= to_sint a < 2^i.
 
 lemma add_corr (a b : W16.t) (a' b' : zmod) (asz bsz : int): 
+   asz < 15 => bsz < 15 =>
    a' = inzmod (W16.to_sint a) =>
    b' = inzmod (W16.to_sint b) =>
    bw16 a asz => 
@@ -47,51 +47,161 @@ lemma add_corr (a b : W16.t) (a' b' : zmod) (asz bsz : int):
      inzmod (W16.to_sint (add a b)) = a' + b' /\
            bw16 (add a b) (max asz bsz + 1).
 admitted.
+(* slow 
+proof
+rewrite /bw16 /add !to_sintE !_smodE => />.
+move => ?? ?? [#?] ?? [#?] ??.
 
-require import Poly_add Array256.
+have bounds_asz : 0 < 2^asz <= 16384; first by split; [ apply gt0_pow2 | move => *; apply (pow_Mle asz 14 _) => /# ].
+have bounds_bsz : 0 < 2^bsz <= 16384; first by split; [ apply gt0_pow2 | move => *; apply (pow_Mle bsz 14 _) => /#].
+have bounds_a : (0 <= to_uint a < 32768) \/ (65536 - 32768 <= to_uint a < 65536); first by smt.
+have bounds_as1 : (0 <= to_uint a < 32768 => 0 <= to_uint a < 2^asz). smt.
+have bounds_as2 : (65536 - 32768 <= to_uint a < 65536 => 65536 -2^asz <= to_uint a < 65536). smt.
+have bounds_b : (0 <= to_uint b < 32768) \/ (65536 - 32768 <= to_uint b < 65536); first by smt.
+have bounds_bs1 : (0 <= to_uint b < 32768 => 0 <= to_uint b < 2^bsz). smt.
+have bounds_bs2 : (65536 - 32768 <= to_uint b < 65536 => 65536 -2^bsz <= to_uint b < 65536). smt.
 
-type pelem = W16.t Array256.t.
+split.
+case(to_uint a + to_uint b < W16.modulus) => /= *.
+rewrite to_uintD_small; first by smt(@W16).
+smt(@ZModP @W16).
 
+rewrite (_: to_uint (a + b) = to_uint a + to_uint b - W16.modulus).
+   have ? : (to_uint a + to_uint b < 2 * W16.modulus). smt.  
+   have ? : (to_uint a + to_uint b = (to_uint a + to_uint b) %% W16.modulus + W16.modulus); smt.
+smt(@ZModP @W16).
+
+split. 
+smt(@IntExtra @W16).
+
+have bound : ((max asz bsz + 1) <= 15); first by  smt().
+have boundd : (2^(max asz bsz + 1) <= 32768); first by smt.  
+have bounddd : (2^asz < 2^(max asz bsz + 1)); first by admit.
+have boundddd : (2^bsz < 2^(max asz bsz + 1)); first by  admit.
+move : bound boundd bounddd boundddd; pose x := 2 ^ (max asz bsz + 1).
+move => *.
+
+elim bounds_a.
+elim bounds_b.
+move => *.
+rewrite to_uintD_small;  by smt(@IntExtra @W16).
+case(to_uint a + to_uint b < W16.modulus) => /= *.
+rewrite to_uintD_small;  by smt(@W16).
+rewrite (_: to_uint (a + b) = to_uint a + to_uint b - W16.modulus).
+   have ? : (to_uint a + to_uint b < 2 * W16.modulus). smt.  
+   have ? : (to_uint a + to_uint b = (to_uint a + to_uint b) %% W16.modulus + W16.modulus); smt.
+smt(@IntExtra @W16).
+
+elim bounds_b.
+move => *.
+case(to_uint a + to_uint b < W16.modulus) => /= *.
+rewrite to_uintD_small;  by smt(@W16).
+rewrite (_: to_uint (a + b) = to_uint a + to_uint b - W16.modulus).
+   have ? : (to_uint a + to_uint b < 2 * W16.modulus). smt.  
+   have ? : (to_uint a + to_uint b = (to_uint a + to_uint b) %% W16.modulus + W16.modulus); smt.
+smt(@IntExtra @W16).
+
+move => *.
+case(to_uint a + to_uint b < W16.modulus) => /= *.
+rewrite to_uintD_small;  by smt(@W16).
+rewrite (_: to_uint (a + b) = to_uint a + to_uint b - W16.modulus).
+   have ? : (to_uint a + to_uint b < 2 * W16.modulus). smt.  
+   have ? : (to_uint a + to_uint b = (to_uint a + to_uint b) %% W16.modulus + W16.modulus); smt.
+smt(@IntExtra @W16).
+
+qed.
+*)
+
+require import NTT_Fq.
+
+clone import NTT_Fq with
+   op ZModP.p <- Fq.q,
+   type ZModP.zmod <- zmod,
+   theory ZModP.Sub <- Sub,
+   op ZModP.inzmod <- inzmod,
+   op ZModP.asint <- asint. (* .. *)
+
+require import Poly_ntt.
 print M.
 
-op repres : pelem -> poly.
+require import Array256.
+import Fq.SignedReductions.
 
-axiom repres_deg pelem :
-      0 <= deg (repres pelem) < 256.
-
-axiom repres_get (p : pelem) (i : int):
-    (repres p).[i] = inzmod (W16.to_sint p.[i]).
-
-op bwpol16 (p : pelem) (sz : int) =
-    all (fun c => bw16 c sz) p axiomatized by bwpol16E.
-
-lemma add_corr aap abp asz bsz:
-   hoare [ M.poly_add :
-      aap = repres ap /\
-      abp = repres bp /\
-      bwpol16 ap asz /\
-      bwpol16 bp bsz ==>
-         repres res = aap + abp /\
-           bwpol16 res (max asz bsz + 1)].
+print M.
+lemma poly_reduct_corr:
+    forall (_a : int Array256.t),
+      phoare[ M.poly_reduce :
+           (forall i, 0<= i < 256 =>
+              (to_sint rp.[i]) = _a.[i]) ==> 
+           forall i, 0<= i < 256 =>
+              to_sint res.[i] = BREDC _a.[i] 26]= 1%r.
 proof.
+move => _a.
 proc.
-unroll for 3.
-wp; skip => />.
-progress.
-rewrite Poly.ext_eq.
-progress.
-rewrite !repres_get.
-case (i0 = 0) => />.
-rewrite add_sem !repres_get.
-move : (add_corr (ap{hr}.[0]) (bp{hr}.[0])
-(inzmod (to_sint ap{hr}.[0])) (inzmod (to_sint bp{hr}.[0])) asz bsz _ _ _ _) => //=.
-move : H; rewrite bwpol16E.
-smt.
-move : H0; rewrite bwpol16E.
-smt.
-admit.
+while (0 <= to_uint j <= 256 /\ 
+       (forall k, 0 <= k < to_uint j => to_sint rp.[k] = (BREDC _a.[k] 26)) /\
+       (forall k, to_uint j <= k < 256 => to_sint rp.[k] =  _a.[k]))
+       (256 - to_uint j) ; last first.
+auto => />. 
+move => &ht H.
+split; first by smt().
+move => *. 
+move : H; rewrite ultE of_uintK => />; smt(@W16 @W64).
+move => *.
+wp. sp.
+exists* t, j.
+elim* => t j.
+print barret_reduct_corr.
+call (barret_reduct_corr _a.[to_uint j]).
+by auto => />;smt(@W64 @Array256).
 qed.
 
+op lift_array (p : W16.t Array256.t) =
+  Array256.map (fun x => inzmod (W16.to_sint x)) p.
 
+op load_array_from_mem(mem : global_mem_t, ptr : W64.t) : W16.t Array256.t.
 
-*)
+axiom load_array_from_memE mem ptr i :
+   0 <= i < 256 =>
+     loadW16 mem (W64.to_uint ptr + 2* i) = (load_array_from_mem mem ptr).[i].
+
+print NTT_Fq.NTT.
+print lift_array_from_mem.
+equiv ntt_correct &m :
+  NTT_Fq.NTT.ntt ~ M.poly_ntt : 
+        r{1} = lift_array rp{2} /\ 
+        zetas{1} = lift_array (load_array_from_mem Glob.mem{2} zetasp{2}) ==> 
+            res{1} = lift_array res{2} /\
+            all (fun x => 0<= W16.to_sint x < 2*Fq.q) res{2}.
+proc.
+seq 3 2 : 
+    (forall k, 0 <= k < 256 => 
+       (-32768 < to_sint rp{2}.[k] < 32768 /\
+       r{1} = lift_array rp{2})); last first.
+exists * r{1}, rp{2}.
+elim* => r1 rp2.
+call {2} (_:  
+     forall i, 0 <= i < 256 =>
+             to_sint rp.[i] = (map (fun (x : W16.t) => to_sint x) rp2).[i]
+     ==> 
+     forall i, 0 <= i < 256 =>
+             to_sint res.[i] =
+             BREDC (map (fun (x : W16.t) => to_sint x) rp2).[i] 26). 
+apply (poly_reduct_corr (Array256.map (fun x => (W16.to_sint x)) rp2)).
+skip. move => &1 &2 [#] ???.
+split.
+move => i ibnd; first by smt (@Array256).
+move => ???.
+split.
++ rewrite (Array256.ext_eq r{1} (lift_array result)) //=.
+   move => x xb;rewrite /lift_array  mapiE //=  (H3 x xb) mapiE => />.
+   move : (BREDCp_corr (to_sint rp2.[x]) 26 _ _ _ _ _);
+      first 5 by smt(@Fq).  
+   move : (H1 x xb);rewrite Array256.tP => [# ] ??? [#] ???.
+   move : (H6 x xb);rewrite /lift_array mapiE => /> *;smt(@ZModP).
++ rewrite allP => i ib />.  
+  rewrite  (H3 i ib) mapiE => />.
+  move : (BREDCp_corr (to_sint rp2.[i]) 26 _ _ _ _ _);smt(@Fq @ZModP).
+admitted.
+
+end KyberPoly.
